RefinedHeap.v
@@ -1,0 +1,400 @@
+Require Import Fiat.ADT Fiat.ADTNotation.
+
+Require Import
+  Coq.Lists.List
+  Coq.Arith.Arith
+  Coq.NArith.NArith
+  Coq.FSets.FMapAVL
+  Coq.FSets.FMapFacts
+  Coq.Structures.OrderedTypeEx
+  Omega.
+
+Module M := FMapAVL.Make(N_as_OT).
+Module F := FMapFacts.Facts M.
+
+Require Import
+  Here.ByteString
+  Here.LibExt
+  Here.Heap.
+
+Require Import
+  Fiat.ADTRefinement
+  Fiat.ADTRefinement.BuildADTRefinements.
+
+Tactic Notation "refine" "method" constr(name) :=
+  match goal with
+    | [ _ : constructorType ?A (consDom {| consID := name
+                                         ; consDom := _ |}) |- _ ] =>
+      idtac "Constructor"
+    | [ _ : methodType ?A (methDom {| methID := name
+                                    ; methDom := _
+                                    ; methCod := _ |})  _ |- _ ] =>
+      idtac "Method"
+    | _ =>
+      fail "Incorrect method name"
+  end.
+
+Generalizable All Variables.
+
+Open Scope N_scope.
+
+Theorem Nle_add_plus : forall n m o, 0 < o -> n <= m -> n <= m + o.
+Proof.
+  intros.
+  rewrite <- (N.add_0_r n).
+  apply N.add_le_mono; nomega.
+Qed.
+
+Theorem Nle_impossible : forall n m, 0 < m -> n + m <= n -> False.
+Proof.
+  intros.
+  rewrite <- (N.add_0_r n) in H0 at 2.
+  apply N.add_le_mono_l in H0.
+  nomega.
+Qed.
+
+Section RefinedHeap.
+
+Variable Word8 : Type.
+Variable Zero : Word8.
+
+Definition MemoryBlock := MemoryBlock Word8.
+Definition HeapSpec    := @HeapSpec Word8 Zero.
+
+Record MemoryBlockC := {
+  memCAddr : N;
+  memCSize : N;
+  memCData : M.t Word8
+}.
+
+Ltac tsubst :=
+  Heap.tsubst;
+  repeat
+    match goal with
+    | [ H : {| memCAddr := _
+             ; memCSize := _
+             ; memCData := _ |} =
+            {| memCAddr := _
+             ; memCSize := _
+             ; memCData := _ |} |- _ ] => inv H
+    end;
+  subst.
+
+Lemma within_reflect : forall x y a,
+  within x y a <-> (x <=? a) && (a <? x + y) = true.
+Proof.
+  intros.
+  unfold within.
+  split; intros; try nomega.
+  apply andb_true_iff; split; nomega.
+Qed.
+
+Theorem Mfind_List_find : forall d base m x,
+  M.find base m = Some x
+    -> base = memCAddr x
+    -> within (memCAddr x) (memCSize x) d
+    -> (forall a b i,
+           M.In (memCAddr a) m ->
+           M.In (memCAddr b) m ->
+           within (memCAddr a) (memCSize a) i ->
+           within (memCAddr b) (memCSize b) i ->
+           a = b)
+    -> List.find (fun p : M.key * MemoryBlockC =>
+                    (fst p =? memCAddr (snd p)) &&
+                    ((memCAddr (snd p) <=? d) &&
+                     (d <? memCAddr (snd p) + memCSize (snd p))))
+                 (M.elements m) = Some (base, x).
+Proof.
+  intros.
+  rewrite F.elements_o in H.
+  setoid_rewrite F.in_find_iff in H2.
+  setoid_rewrite F.elements_o in H2.
+  generalize dependent base.
+  induction (M.elements (elt:=MemoryBlockC) m); simpl in *.
+    discriminate.
+  destruct a; simpl in *; intros.
+  unfold F.eqb, M.E.eq_dec in H.
+  destruct (N.eq_dec base k); subst; inv H.
+    rewrite N.eqb_refl, andb_true_l.
+    apply within_reflect in H1.
+    setoid_rewrite H1.
+    reflexivity.
+  decisions.
+    apply andb_true_iff in Heqe.
+    destruct Heqe.
+    apply within_reflect in H0.
+    specialize (H2 m0 x k).
+    apply N.eqb_eq in H; subst.
+    (* jww (2016-06-24): I need a way of knowing that if two memory blocks
+       overlap the same point, they must be the same block. *)
+    admit.
+  apply IHl; intros.
+  - eapply H2.
+    + unfold F.eqb, M.E.eq_dec.
+      destruct (N.eq_dec (memCAddr a) k).
+        unfold not; intros; discriminate.
+      exact H.
+    + unfold F.eqb, M.E.eq_dec.
+      destruct (N.eq_dec (memCAddr b) k).
+        unfold not; intros; discriminate.
+      exact H0.
+    + exact H4.
+    + exact H5.
+  - exact H3.
+  - reflexivity.
+Admitted.
+
+Lemma HeapImpl : FullySharpened HeapSpec.
+Proof.
+  start sharpening ADT.
+  hone representation using
+    (fun (or : Ensemble MemoryBlock) (nr : N * M.t MemoryBlockC) =>
+       ADTInduction.fromADT HeapSpec or /\
+       forall addr size,
+         (forall data,
+            In _ or {| memAddr := addr
+                     ; memSize := size
+                     ; memData := data |} ->
+            (addr + size <= fst nr /\
+             exists cdata,
+               M.find addr (snd nr)
+                 = Some {| memCAddr := addr
+                         ; memCSize := size
+                         ; memCData := cdata |} /\
+               (forall i v, In _ data (i, v) <-> M.find i cdata = Some v))) /\
+         (forall cdata,
+             M.find addr (snd nr)
+               = Some {| memCAddr := addr
+                       ; memCSize := size
+                       ; memCData := cdata |} ->
+             (addr + size <= fst nr /\
+              exists data,
+                In _ or {| memAddr := addr
+                         ; memSize := size
+                         ; memData := data |} /\
+                (forall i v, In _ data (i, v) <-> M.find i cdata = Some v)))).
+
+  refine method emptyS.
+  {
+    simplify with monad laws.
+    refine pick val (0%N, @M.empty _).
+      finish honing.
+    split; intros.
+      apply ADTInduction.fromADTConstructor with (cidx:=Fin.F1).
+      constructor.
+    simpl; split; intros.
+      inv H0.
+    apply F.find_mapsto_iff, F.empty_mapsto_iff in H0.
+    contradiction.
+  }
+
+  refine method allocS.
+  {
+    unfold find_free_block.
+    simplify with monad laws.
+    refine pick val (fst r_n).
+      simplify with monad laws.
+      refine pick val (fst r_n + proj1_sig d,
+                       M.add (fst r_n)
+                             {| memCAddr := fst r_n
+                              ; memCSize := proj1_sig d
+                              ; memCData := M.empty _ |}
+                             (snd r_n)).
+        simplify with monad laws; simpl.
+        finish honing.
+      clear H.
+      destruct H0.
+      split; intros.
+        apply ADTInduction.fromADTMethod
+          with (midx:=Fin.F1) (r:=r_o); trivial.
+        exists d.
+        exists (fst r_n).
+        simpl.
+        apply BindComputes with (a:=fst r_n).
+          unfold find_free_block.
+          apply PickComputes; intros.
+          unfold found_block_at_base in H1.
+          destruct (H0 addr' len') as [H2 _]; clear H0.
+          destruct (H2 data' H1) as [H3 _]; clear H2.
+          unfold overlaps.
+          nomega.
+        reflexivity.
+      simpl; split; intros.
+        apply Add_inv in H1.
+        destruct H1.
+          destruct (H0 addr size) as [? ?]; clear H0;
+          destruct (H2 data H1) as [? ?].
+          split.
+            destruct d; simpl.
+            apply Nle_add_plus; trivial.
+          destruct H4.
+          exists x.
+          split; intros.
+            apply F.find_mapsto_iff, F.add_mapsto_iff.
+            right.
+            split.
+              destruct H4.
+              destruct (H3 _ H4).
+              destruct H7.
+              destruct H7.
+              pose proof (allocations_have_size H _ _ _ H7).
+              clear -H0 H9.
+              unfold not; intros; subst.
+              eapply Nle_impossible; eassumption.
+            apply F.find_mapsto_iff.
+            apply H4.
+          apply H4.
+        tsubst.
+        split; intros.
+          nomega.
+        exists (M.empty Word8).
+        split; intros.
+          apply F.find_mapsto_iff, F.add_mapsto_iff.
+          left; tauto.
+        split; intros.
+          inv H1.
+        apply F.find_mapsto_iff, F.empty_mapsto_iff in H1.
+        contradiction.
+      apply F.find_mapsto_iff in H1.
+      apply F.add_mapsto_iff in H1.
+      destruct H1; destruct H1; tsubst.
+        split; intros.
+          nomega.
+        destruct (H0 (fst r_n) (` d)).
+        eexists.
+        split; intros.
+          right; constructor.
+        split; intros.
+          inv H3.
+        apply F.find_mapsto_iff, F.empty_mapsto_iff in H3.
+        contradiction.
+      apply F.find_mapsto_iff in H2.
+      destruct (H0 addr size); clear H0.
+      destruct (H4 _ H2).
+      destruct d; simpl in *.
+      split; intros.
+        apply Nle_add_plus; trivial.
+      destruct H5.
+      exists x0.
+      split; intros.
+        left.
+        apply H5.
+      apply H5.
+    clear H.
+    unfold found_block_at_base.
+    intros.
+    destruct H0.
+    destruct (H1 addr' len'); clear H1.
+    destruct (H2 _ H).
+    unfold overlaps.
+    nomega.
+  }
+
+  refine method freeS.
+  {
+    unfold free_block.
+    simplify with monad laws; simpl.
+    refine pick val (fst r_n, M.remove d (snd r_n)).
+      simplify with monad laws; simpl.
+      finish honing.
+    destruct H0; simpl in *.
+    split; intros.
+      apply ADTInduction.fromADTMethod
+        with (midx:=Fin.FS (Fin.F1)) (r:=r_o); trivial.
+      exists d.
+      exists tt.
+      simpl.
+      constructor.
+    unfold free_block.
+    split; intros.
+      destruct (H1 addr size); clear H1 H4.
+      inv H2.
+      destruct (H3 _ H1).
+      split; intros; trivial.
+      destruct H5.
+      exists x.
+      split; intros.
+        rewrite F.remove_neq_o.
+          apply H5.
+        unfold Ensembles.In in H4.
+        exact H4.
+      apply H5.
+    destruct (H1 addr size); clear H1 H3.
+    apply F.find_mapsto_iff in H2.
+    apply F.remove_mapsto_iff in H2.
+    destruct H2.
+    apply F.find_mapsto_iff in H2.
+    destruct (H4 _ H2); clear H2 H4.
+    split; trivial.
+    destruct H5.
+    exists x.
+    split.
+      constructor.
+        apply H2.
+      unfold not; intros.
+      unfold Ensembles.In in H4; simpl in H4; subst.
+      tauto.
+    apply H2.
+  }
+
+  refine method reallocS.
+  {
+    admit.
+  }
+
+  refine method peekS.
+  {
+    unfold found_block.
+    simplify with monad laws; simpl.
+    refine pick val
+      (Ifopt List.find (fun p =>
+                          let blk := snd p in
+                          (* jww (2016-06-24): Unnecessarily inefficient *)
+                          (fst p =? memCAddr (snd p)) &&
+                          Decidable.Decidable_witness
+                            (P:=within (memCAddr blk) (memCSize blk) d))
+                       (M.elements (snd r_n)) as p
+       Then let blk := snd p in
+            Ifopt M.find (d - memCAddr blk) (memCData blk) as v
+            Then v
+            Else Zero
+       Else Zero).
+      simplify with monad laws; simpl.
+      refine pick val r_n.
+        simplify with monad laws; simpl.
+        unfold If_Opt_Then_Else; simpl.
+        finish honing.
+      apply H0.
+    intros; simpl; clear H.
+    destruct H0, H1.
+    destruct (H0 base len'); clear H4.
+    destruct (H3 _ H1); clear H3.
+    destruct H5.
+    destruct H3.
+    rewrite Mfind_List_find
+      with (base:=base)
+           (x:={| memCAddr := base
+                ; memCSize := len'
+                ; memCData := x |}); simpl; trivial.
+      destruct (M.find (elt:=Word8) (d - base) x) eqn:Heqe; simpl.
+        left; apply H5; assumption.
+      right; reflexivity.
+    admit.
+  }
+
+  refine method pokeS.
+  {
+    admit.
+  }
+
+  refine method memcpyS.
+  {
+    admit.
+  }
+
+  refine method memsetS.
+  {
+    admit.
+  }
+  finish_SharpeningADT_WithoutDelegation.
+Abort.
